%%%%%%%%%%%%%%%%%%%%%%%%%%%%%%%%%%%%%%%%%%%%%%%%%%%%%%%%%%%%%%%%%%%%%%%%%%%%%%%%%%%%%%%%%%%%%%%%%%%%%%%%%%%%%%%%%%%%%%%%%%%%%%%%%%%%%%%%%%%%%%%%%%%%%%%%%%%%%%%%%%%%%%%%%%%%%%%%%%%%%%%%%%%%
% Written By Michael Brodskiy
% Class: Differential Equations (MATH-294)
% Professor: M. Shah
%%%%%%%%%%%%%%%%%%%%%%%%%%%%%%%%%%%%%%%%%%%%%%%%%%%%%%%%%%%%%%%%%%%%%%%%%%%%%%%%%%%%%%%%%%%%%%%%%%%%%%%%%%%%%%%%%%%%%%%%%%%%%%%%%%%%%%%%%%%%%%%%%%%%%%%%%%%%%%%%%%%%%%%%%%%%%%%%%%%%%%%%%%%%

\documentclass[12pt]{article} 
\usepackage{alphalph}
\usepackage[utf8]{inputenc}
\usepackage[russian,english]{babel}
\usepackage{titling}
\usepackage{amsmath}
\usepackage{graphicx}
\usepackage{enumitem}
\usepackage{amssymb}
\usepackage[super]{nth}
\usepackage{everysel}
\usepackage{ragged2e}
\usepackage{geometry}
\usepackage{fancyhdr}
\usepackage{cancel}
\usepackage{siunitx}
\geometry{top=1.0in,bottom=1.0in,left=1.0in,right=1.0in}
\newcommand{\subtitle}[1]{%
  \posttitle{%
    \par\end{center}
    \begin{center}\large#1\end{center}
    \vskip0.5em}%

}
\usepackage{hyperref}
\hypersetup{
colorlinks=true,
linkcolor=blue,
filecolor=magenta,      
urlcolor=blue,
citecolor=blue,
}

\urlstyle{same}


\title{Differential Equations $-$ Final Exam}
\date{\today}
\author{Michael Brodskiy\\ \small Professor: Meetal Shah}

% Mathematical Operations:

% Sum: $$\sum_{n=a}^{b} f(x) $$
% Integral: $$\int_{lower}^{upper} f(x) dx$$
% Limit: $$\lim_{x\to\infty} f(x)$$

\begin{document}

\maketitle

\hline
\begin{equation}
  \begin{split}
    I=e^{-\int\,dx}\\
    I=e^{-x}\\
    e^{-x}y=\int xe^{-x}\\
    e^{-x}y=-xe^{-x}-e^{-x}+c\\
    y=-x-1+ce^{x}\\
    \text{The region is the whole $xy$-plane}
  \end{split}
  \label{1}
\end{equation}
\hline

\begin{equation}
  \begin{split}
    \frac{dy}{dx}=-2xy^2\\
    \frac{1}{y^2}\,dy=-2x\,dx\\
    \int\frac{1}{y^2}\,dy=\int-2x\,dx\\
    -\frac{1}{y}=-x^2+c\\
    y=\frac{1}{x^2+c}
  \end{split}
  \label{2}
\end{equation}

\hline
\begin{equation}
  \begin{split}
    L_1\frac{di_2}{dt}+(R_1+R_2)i_2+R_1i_3=E(t)\\
    L_2\frac{di_3}{dt}+(R_1+R_3)i_3+R_1i_2=E(t)\\
  \end{split}
  \label{3}
\end{equation}

\hline
\begin{equation}
  \begin{split}
    \frac{d^2y}{d\theta^2}+y=0\\
    m^2+1=0\\
    m=\pm i\\
    y=e^{0\theta}\left( c_1\sin\left( \theta \right)+c_2\cos\left( \theta \right) \right)\\
    y= c_1\sin\left( \theta \right)+c_2\cos\left( \theta \right)\\
    y\left( \frac{\pi}{3} \right)=\frac{c_1\sqrt{3}}{2}+\frac{c_2}{2}=0\\
    y'\left( \frac{\pi}{3} \right)=\frac{c_1}{2}-\frac{c_2\sqrt{3}}{2}=2\\
    c_1\sqrt{3}+c_2=0\\
    c_1-c_2\sqrt{3}=4\\
    c_1=1,\,\,\,c_2=-\sqrt{3}\\
    y=\sin(\theta)-\sqrt{3}\cos(\theta)\\
  \end{split}
  \label{4}
\end{equation}

\hline
\begin{equation}
  \begin{split}
    m^2-16=0\\
    m=\pm4\\
    y=c_1e^{-4x}+c_2e^{4x}+\dots\\
    y_p(x)=(Ax+B)e^{4x}\\
    y_p'(x)=Ae^{4x}+4Axe^{4x}+4Be^{4x}\\
    y_p''(x)=8Ae^{4x}+16Axe^{4x}+16Be^{4x}\\
    8Ae^{4x}=2e^{4x}\\
    A=\frac{1}{4}\\
    y=c_1e^{-4x}+c_2e^{4x}+\frac{1}{4}xe^{4x}
  \end{split}
  \label{5}
\end{equation}
\hline
\newpage

\hline

\begin{equation}
  \begin{split}
    k=5\\
    m=\frac{1}{4}\\
    D^2x+4Dx+20x=0\\
    \lambda^2-\omega^2=-16\\
    A=\sqrt{\omega^2-\lambda^2}=4\\
    x(t)=e^{-2t}\left(c_1\cos\left( 4t \right)+c_2\sin\left( 4t \right) \right)\\
    c_1=\frac{1}{2}\\
    x'(0)\longrightarrow -1+4c_2=2\\
    c_2=\frac{3}{4}\\
    x(t)=e^{-2t}\left(\frac{1}{2}\cos\left( 4t \right)+\frac{3}{4}\sin\left( 4t \right) \right)\\
  \end{split}
  \label{6}
\end{equation}
\hline


\begin{equation}
  \begin{split}
    x^2-2x+10=0\\
    x=1\pm 3i\\
    x_1=\sqrt{(1-0)^2+(3-0)^2}=\sqrt{10}\\
    x_2=\sqrt{(1-1)^2+(3-0)^2}=3\\
  \end{split}
  \label{7}
\end{equation}
\hline

\begin{equation}
  \begin{split}
    f(t)=1-2\mathcal{U}\left( t-a \right)\\
    \mathcal{L}\left\{ y'+y=f(t) \right\}=sF(s)+F(s)=\frac{1}{s}-\frac{2e^{-s}}{s}\\
    F(s)=\frac{1}{s(s+1)}-\frac{2e^{-s}}{s(s+1)}\\
    \mathcal{L}^{-1}\left\{  \frac{1}{s(s+1)}\right\}=-(e^{-t}-1)\\
    \mathcal{L}^{-1}\left\{  -\frac{2e^{-s}}{s(s+1)}\right\}=2(e^{-(t-1)}-1)\mathcal{U}(t-1)\\
  f(t)=-e^{-t}+1+(2e^{-(t-1)}-2)\mathcal{U}(t-1)
  \end{split}
  \label{8}
\end{equation}


\hline
\begin{equation}
  \begin{split}
    |\bold{A}-\lambda\bold{I}|=\begin{pmatrix} -6-\lambda & 2 \\ -3 & 1-\lambda \\ \end{pmatrix}\\
    \lambda^2+5\lambda=0\\
    \lambda_n=-5,0\\
    \text{When }\lambda_n=-5\\
    \begin{vmatrix} -1 & 2 \\ -3 & 6 \\ \end{vmatrix}\\
    k_1=2,\,\,\,k_2=1\\
    \text{When }\lambda_n=0\\
    \begin{vmatrix} -6 & 2 \\ -3 & 1 \\ \end{vmatrix}\\
    k_1=1,\,\,\,k_2=3\\
    \bold{X}=c_1\begin{pmatrix} 2 \\ 1 \end{pmatrix}e^{-5t}+c_2\begin{pmatrix} 1 \\ 3 \end{pmatrix}
  \end{split}
  \label{9}
\end{equation}

\hline
\begin{equation}
  \begin{split}
    y^{(5)}(c)\cdot\frac{h^5}{5!}\\
    y^{(5)}(x)=2^5e^{2x}\\
    0\leq c\leq .1\\
    2^5e^{\frac{1}{5}}\cdot\frac{.1^5}{120}=\frac{e^{\frac{1}{5}}}{375000}\\
  \end{split}
  \label{10}
\end{equation}
\hline

\begin{equation}
  \begin{split}
    Odd\cdot Even=Odd\\
    b_n=2\int_0^1 x|x|\sin\left( n\pi x \right)\,dx\\
    b_n=2\cdot\frac{2x^2\sin(n\pi x)+(2x-x^3)\cos(n\pi x)}{n^2\pi^2|x|}\Big|_0^1\\
    b_n=\frac{2(-1)^n}{n^2\pi^2}\\
    a_0=0\\
    a_n=0\\
    y(x)=\sum_{n=1}^{\infty}\frac{2(-1)^n}{n^2\pi^2}\sin(n\pi x)
  \end{split}
  \label{11}
\end{equation}
\hline

\end{document}

