%%%%%%%%%%%%%%%%%%%%%%%%%%%%%%%%%%%%%%%%%%%%%%%%%%%%%%%%%%%%%%%%%%%%%%%%%%%%%%%%%%%%%%%%%%%%%%%%%%%%%%%%%%%%%%%%%%%%%%%%%%%%%%%%%%%%%%%%%%%%%%%%%%%%%%%%%%%%%%%%%%%%%%%%%%%%%%%%%%%%%%%%%%%%
% Written By Michael Brodskiy
% Class: Differential Equations (MATH-294)
% Professor: M. Shah
%%%%%%%%%%%%%%%%%%%%%%%%%%%%%%%%%%%%%%%%%%%%%%%%%%%%%%%%%%%%%%%%%%%%%%%%%%%%%%%%%%%%%%%%%%%%%%%%%%%%%%%%%%%%%%%%%%%%%%%%%%%%%%%%%%%%%%%%%%%%%%%%%%%%%%%%%%%%%%%%%%%%%%%%%%%%%%%%%%%%%%%%%%%%

\documentclass[12pt]{article} 
\usepackage{alphalph}
\usepackage[utf8]{inputenc}
\usepackage[russian,english]{babel}
\usepackage{titling}
\usepackage{amsmath}
\usepackage{graphicx}
\usepackage{enumitem}
\usepackage{amssymb}
\usepackage[super]{nth}
\usepackage{everysel}
\usepackage{ragged2e}
\usepackage{geometry}
\usepackage{multicol}
\usepackage{fancyhdr}
\usepackage{cancel}
\usepackage{siunitx}
\geometry{top=1.0in,bottom=1.0in,left=1.0in,right=1.0in}
\newcommand{\subtitle}[1]{%
  \posttitle{%
    \par\end{center}
    \begin{center}\large#1\end{center}
    \vskip0.5em}%

}
\usepackage{hyperref}
\hypersetup{
colorlinks=true,
linkcolor=blue,
filecolor=magenta,      
urlcolor=blue,
citecolor=blue,
}

\urlstyle{same}
\usepackage{fancyhdr}
\pagestyle{fancy}
\lhead[\textsc{Fall 2020}]{\textsc{Fall 2020}}
\chead[\textit{Differential Equations Final Exam Equation Sheet}]{\textit{Differential Equations Final Exam Equation Sheet}}
\rhead[\textsc{Math-294}]{\textsc{Math-294}}
\cfoot[\thepage]{\thepage}


% Mathematical Operations:

% Sum: $$\sum_{n=a}^{b} f(x) $$
% Integral: $$\int_{lower}^{upper} f(x) dx$$
% Limit: $$\lim_{x\to\infty} f(x)$$

\begin{document}
  \begin{center}
    \Small\vline\textbf{\underline{$\overline{\text{Good luck. May the $\bold{+c}$ be with you.}}$}}\Small\vline
  \end{center}
  \vspace{-30pt}

\begin{multicols}{2}

  \begin{equation*}
    \begin{split}
      L\frac{d^2q}{dt^2}+R\frac{dq}{dt}+q\frac{1}{C}=E(t)\\
      \text{If }R\neq0\text{ then }q_c(t)\text{ is transient}\\
      E(t)\text{ is }\cos,\,\sin,\,c\rightarrow q_p(t)\text{is steady-state}\\
      \end{split}
    \label{1}
  \end{equation*}

  \begin{equation*}
    \begin{split}
      D^n;\,x^{n-1}\\
      (D-\alpha)^n;\,x^{n-1}e^{\alpha x}\\
      [D^2-2\alpha D+\alpha^2+\beta^2]^n;\,x^{n-1}e^{\alpha x}\cos\beta x
    \end{split}
    \label{2}
  \end{equation*}

\end{multicols}

\begin{multicols}{2}

\begin{equation*}
  \begin{split}
    \underline{f(t)}\,\,\,\,&\vline\,\,\,\,\underline{F(s)}\\
      1\,\,\,\,&\vline\,\,\,\,\frac{1}{s}\\
      t^n\,\,\,\,&\vline\,\,\,\,\frac{n!}{s^{n+1}}\\
      t^{-\frac{1}{2}}\,\,\,\,&\vline\,\,\,\,\sqrt{\frac{\pi}{s}}\\
      t^{\frac{1}{2}}\,\,\,\,&\vline\,\,\,\,\frac{\sqrt{\pi}}{2s^{\frac{3}{2}}}\\
      \sin (kt)\,\,\,\,&\vline\,\,\,\,\frac{k}{s^2+k^2}\\
      \cos (kt)\,\,\,\,&\vline\,\,\,\,\frac{s}{s^2+k^2}\\
      \sin^2(kt)\,\,\,\,&\vline\,\,\,\,\frac{2k^2}{s(s^2+4k^2)}\\
      \cos^2(kt)\,\,\,\,&\vline\,\,\,\,\frac{s^2+2k^2}{s(s^2+4k^2)}\\
      e^{\alpha t}\,\,\,\,&\vline\,\,\,\,\frac{1}{s-a}\\
    \sinh (kt)\,\,\,\,&\vline\,\,\,\,\frac{k}{s^2-k^2}\\
    \cosh (kt)\,\,\,\,&\vline\,\,\,\,\frac{s}{s^2-k^2}\\
      \sinh^2 (kt)\,\,\,\,&\vline\,\,\,\,\frac{2k^2}{s(s^2-4k^2)}\\
      \cosh^2 (kt)\,\,\,\,&\vline\,\,\,\,\frac{s^2-2k^2}{s(s^2-4k^2)}\\
    t\sin(kt)\,\,\,\,&\vline\,\,\,\,\frac{2ks}{(s^2+k^2)^2}\\
    t\cos(kt)\,\,\,\,&\vline\,\,\,\,\frac{s^2-k^2}{(s^2+k^2)^2}\\
    \sin(kt)+kt\cos(kt)\,\,\,\,&\vline\,\,\,\,\frac{2ks^2}{(s^2+k^2)^2}\\
    \sin(kt)-kt\cos(kt)\,\,\,\,&\vline\,\,\,\,\frac{2k^3}{(s^2+k^2)^2}\\
    \delta(t-t_0)\,\,\,\,&\vline\,\,\,\,e^{-st_0}
  \end{split}
  \label{3}
  \end{equation*}
    
\begin{equation*}
  \begin{split}
    \underline{f(t)}\,\,&\vline\,\,\underline{F(s)}\\
    t\sinh(kt)\,\,&\vline\,\,\frac{2ks}{(s^2-k^2)^2}\\
    t\cosh(kt)\,\,&\vline\,\,\frac{s^2+k^2}{(s^2-k^2)^2}\\
    \frac{e^{at}-e^{bt}}{a-b}\,\,&\vline\,\,\frac{1}{(s-a)(s-b)}\\
    \frac{ae^{at}-be^{bt}}{a-b}\,\,&\vline\,\,\frac{s}{(s-a)(s-b)}\\
    1-\cos(kt)\,\,&\vline\,\,\frac{k^2}{s(s^2+k^2)}\\
    kt-\sin(kt)\,\,&\vline\,\,\frac{k^3}{s^2(s^2+k^2)}\\
    \frac{a\sin(bt)-b\sin(at)}{ab(a^2-b^2)}\,\,&\vline\,\,\frac{1}{(s^2+a^2)(s^2+b^2)}\\
    \frac{\cos(bt)-\cos(at)}{a^2-b^2}\,\,&\vline\,\,\frac{s}{(s^2+a^2)(s^2+b^2)}\\
    \sin(kt)\sinh(kt)\,\,&\vline\,\,\frac{2k^2s}{s^4+4k^4}\\
    \sin(kt)\cosh(kt)\,\,&\vline\,\,\frac{k(s^2+2k^2)}{s^4+4k^4}\\
    \cos(kt)\sinh(kt)\,\,&\vline\,\,\frac{k(s^2-2k^2)}{s^4+4k^4}\\
    \cos(kt)\cosh(kt)\,\,&\vline\,\,\frac{s^3}{s^4+4k^4}\\
    \frac{e^{bt}-e^{at}}{t}\,\,&\vline\,\,\ln\left(\frac{s-a}{s-b}\right)\\
    e^{at}f(t)\,\,&\vline\,\,F(s-a)\\
    \mathcal{U}(t-a)\,\,&\vline\,\,\frac{e^{-as}}{s}\\
    f(t-a)\mathcal{U}(t-a)\,\,&\vline\,\,e^{-as}F(s)\\
    f\ast g=\int_0^t f(\tau)g(t-\tau)\,d\tau\,\,&\vline\,\,F(s)G(s)\\
    g(t)\mathcal{U}(t-a)\,\,&\vline\,\,e^{-as}\mathcal{L}\left\{ g(t+a) \right\}\\
  \end{split}
  \label{4}
  \end{equation*}

\end{multicols}

\begin{multicols}{2}

  \begin{equation*}
    \begin{split}
      \frac{d^2x}{dt^2}+\frac{\beta}{m}\frac{dx}{dt}+\frac{k}{m}x=f(t)\\
      \lambda^2-\omega^2>0\\
      m_{1,2}=-\lambda \pm\sqrt{\lambda^2-\omega^2}\\
      x(t)=e^{-\lambda t}\left(c_1e^{\sqrt{\lambda^2-\omega^2}t}+c_2e^{-\sqrt{\lambda^2-\omega^2}} \right)\\
    \end{split}
    \label{5}
  \end{equation*}

  \begin{equation*}
    \begin{split}
      2\lambda=\frac{\beta}{m}\text{ and } \omega^2=\frac{k}{m}\\ 
     \lambda^2-\omega^2=0\\
      m_{1,2}=0\\
      x(t)=e^{-\lambda t}(c_1+c_2t)\\
    \end{split}
    \label{6}
  \end{equation*}

\end{multicols}
  \vspace{-20pt}

\begin{multicols}{2}

  \begin{equation*}
    \begin{split}
      F=kx\\
      m\frac{d^2x}{dt^2}+2\lambda\frac{dx}{dt}+\omega^2x=f(t)\\
      \lambda^2-\omega^2<0\\
      m_{1,2}=-\lambda \pm\sqrt{\omega^2-\lambda^2}i\\
      A=\sqrt{\omega^2-\lambda^2}\\
      x(t)=e^{-\lambda t}\left(c_1\cos At+c_2\sin At\right)\\
    \end{split}
    \label{7}
  \end{equation*}

  \begin{equation*}
    \begin{split}
      W=mg\\
      \text{Spring Parallel: } k_eff=k_1+k_2\\
      \text{Spring Series: } k_eff=\frac{k_1k_2}{k_1+k_2}\\
    \frac{d^2x}{dt^2}+\omega^2x=0\\
    x(t)=c_1\cos\omega t+ c_2\sin\omega t\\
    =A\sin(\omega t+\phi)
    \end{split}
    \label{8}
  \end{equation*}


\end{multicols}
  \vspace{-20pt}

\begin{multicols}{2}

  \begin{equation*}
    \begin{split}
      \text{Given }a_2(x)\frac{d^2y}{dx^2}+a_1(x)\frac{dy}{dx}+a_0(x)y=0\\
      \text{Has radius of convergence given by distance}\\
      \text{from analysis point to roots of } a_2(x)\\
      y=\sum_{n=0}^{\infinity} c_nx^n\\
      y'=\sum_{n=1}^{\infinity} nc_nx^{n-1}\\
      y''=\sum_{n=2}^{\infinity} n(n-1)c_nx^{n-2}\\
    \end{split}
    \label{9}
  \end{equation*}

  \begin{equation*}
    \begin{split}
      k_1=f\left(x,y\right)\\
      k_2=f\left(x+\frac{h}{2},y+\frac{h\cdot k_1}{2}\right)\\
      k_3=f\left(x+\frac{h}{2},y+\frac{h\cdot k_2}{2}\right)\\
      k_4=f\left(x+h,y+h\cdot k_3\right)\\
      RK4=y+h\left( \frac{k_1}{6}+\frac{k_2}{3}+\frac{k_3}{3}+\frac{k_4}{6} \right)\\
      O(h^n)=y^{(n)}\left( c \right)&\frac{h^n}{n!}\\
      O(h^4)\text{ for global &truncation on } RK4\\
      O(h^5)\text{ for local &truncation on } RK4\\
    \end{split}
    \label{10}
  \end{equation*}

\end{multicols}

\begin{multicols}{2}

  \begin{equation*}
    \begin{split}
      \text{Even if } f(-x)=f(x)\\
      \text{Even }=\text{ Cosine Series}\\
      f(x)=\frac{a_0}{2}+\sum_{n=1}^{\infty}a_n\cos\frac{n\pi}{p}x\\
      a_0=\frac{2}{p}\int_0^pf(x)\,dx\\
      a_n=\frac{2}{p}\int_0^pf(x)\cos\frac{n\pi}{p}x\,dx\\
      b_n=0\\
    \end{split}
    \label{11}
  \end{equation*}

  \begin{equation*}
    \begin{split}
      \text{Odd if } f(-x)=-f(x)\\
      \text{Odd }=\text{ Sine Series}\\
      f(x)=\sum_{n=1}^{\infty}b_n\sin\frac{n\pi}{p}x\\
      a_0=0\\
      a_n=0\\
      b_n=\frac{2}{p}\int_0^pf(x)\sin\frac{n\pi}{p}x\,dx\\
    \end{split}
    \label{12}
  \end{equation*}


\end{multicols}

\end{document}

